Risc0/Gadgets/ComputeDecode/Constraints/WeakestPresPart7.lean
@@ -9,7 +9,28 @@ open MLIRNotation
 
 -- The state obtained by running Code.part7 on st
 def part7_state (st: State) : State :=
-  sorry
+  
+        ((((st[felts][{ name := "%34" }] ←
+                Option.get! (State.felts st { name := "%33" }) *
+                  Option.get! (State.felts st { name := "%3" }))["%35"] ←ₛ
+              getImpl st { name := "data" } (0 : Back) (12 : ℕ))[felts][{ name := "%36" }] ←
+            Option.get!
+                (State.felts
+                  ((st[felts][{ name := "%34" }] ←
+                      Option.get! (State.felts st { name := "%33" }) *
+                        Option.get! (State.felts st { name := "%3" }))["%35"] ←ₛ
+                    getImpl st { name := "data" } (0 : Back) (12 : ℕ))
+                  { name := "%35" }) *
+              Option.get! (State.felts st { name := "%2" }))[felts][{ name := "%37" }] ←
+          Option.get!
+                (State.felts
+                  ((st[felts][{ name := "%34" }] ←
+                      Option.get! (State.felts st { name := "%33" }) *
+                        Option.get! (State.felts st { name := "%3" }))["%35"] ←ₛ
+                    getImpl st { name := "data" } (0 : Back) (12 : ℕ))
+                  { name := "%35" }) *
+              Option.get! (State.felts st { name := "%2" }) +
+            Option.get! (State.felts st { name := "%33" }) * Option.get! (State.felts st { name := "%3" })) 
 
 def part7_drops (st: State) : State :=
   State.dropFelts (State.dropFelts (State.dropFelts (State.dropFelts (State.dropFelts (State.dropFelts (st) ⟨"%2"⟩) ⟨"%3"⟩) ⟨"%33"⟩) ⟨"%34"⟩) ⟨"%35"⟩) ⟨"%36"⟩
@@ -26,15 +47,43 @@ lemma part7_wp {st : State} :
   generalize eq : (dropfelt ⟨"%2"⟩;dropfelt ⟨"%3"⟩;dropfelt ⟨"%33"⟩;dropfelt ⟨"%34"⟩;dropfelt ⟨"%35"⟩;dropfelt ⟨"%36"⟩;Code.part8;dropfelt ⟨"%31"⟩;dropfelt ⟨"%37"⟩;dropfelt ⟨"%32"⟩;dropfelt ⟨"%38"⟩;dropfelt ⟨"%39"⟩;Code.part9;dropfelt ⟨"%40"⟩;dropfelt ⟨"%29"⟩;dropfelt ⟨"%41"⟩;dropfelt ⟨"%9"⟩;Code.part10;dropfelt ⟨"%42"⟩;dropfelt ⟨"%45"⟩;Code.part11;dropfelt ⟨"%4"⟩;dropfelt ⟨"%1"⟩;dropfelt ⟨"%48"⟩;dropfelt ⟨"%49"⟩;dropfelt ⟨"%47"⟩;dropfelt ⟨"%50"⟩;Code.part12;dropfelt ⟨"%51"⟩;dropfelt ⟨"%52"⟩;dropfelt ⟨"%53"⟩;Code.part13;dropfelt ⟨"%46"⟩;dropfelt ⟨"%54"⟩;dropfelt ⟨"%55"⟩;dropfelt ⟨"%44"⟩;Code.part14;dropfelt ⟨"%0"⟩;dropfelt ⟨"%56"⟩;dropfelt ⟨"%8"⟩;dropfelt ⟨"%57"⟩;dropfelt ⟨"%60"⟩;Code.part15;dropfelt ⟨"%61"⟩;dropfelt ⟨"%59"⟩;dropfelt ⟨"%62"⟩;dropfelt ⟨"%7"⟩;Code.part16;dropfelt ⟨"%6"⟩;dropfelt ⟨"%28"⟩;dropfelt ⟨"%43"⟩;dropfelt ⟨"%58"⟩;dropfelt ⟨"%63"⟩;dropfelt ⟨"%64"⟩) = prog
   unfold Code.part7
   MLIR
+  rewrite [←eq]
+  rewrite [MLIR.run_seq_def,MLIR.run_dropfelt, MLIR.run_seq_def,MLIR.run_dropfelt, MLIR.run_seq_def,MLIR.run_dropfelt, MLIR.run_seq_def,MLIR.run_dropfelt, MLIR.run_seq_def,MLIR.run_dropfelt, MLIR.run_seq_def,MLIR.run_dropfelt]
+  unfold part7_state_update part7_drops part7_state
+  rfl
 
 lemma part7_updates_opaque {st : State} : 
   Code.getReturn (part6_state_update st) ↔
   Code.getReturn (part7_state_update (part6_drops (part6_state st))) := by
   simp [part6_state_update, part7_wp]
 
-lemma part7_cumulative_wp {x0 y0 y1 y2 y3 y4 y5 y6 y7 y8 y9 y10 y11 y12 y13 y14 y15 y16 y17 y18 y19: Felt} :
-  Code.run (start_state [x0] ([y0,y1,y2,y3,y4,y5,y6,y7,y8,y9,y10,y11,y12,y13,y14,y15,y16,y17,y18,y19])) ↔
-  sorry := by
+lemma part7_cumulative_wp {x0 x1 x2 x3 y0 y1 y2 y3 y4 y5 y6 y7 y8 y9 y10 y11 y12 y13 y14 y15 y16 y17: Felt} :
+  Code.run (start_state [x0,x1,x2,x3] ([y0,y1,y2,y3,y4,y5,y6,y7,y8,y9,y10,y11,y12,y13,y14,y15,y16,y17])) ↔
+  Code.getReturn
+      (part7_state_update
+        (((((((({
+                          buffers :=
+                            ((fun x => Map.empty x)[{ name := "data" }] ←ₘ
+                                [[some y0, some y1, some y2, some y3, some y4, some y5, some y6, some y7, some y8,
+                                    some y9, some y10, some y11, some y12, some y13, some y14, some y15, some y16,
+                                    some y17]])[{ name := "in" }] ←ₘ
+                              [[some x0, some x1, some x2, some x3]],
+                          bufferWidths :=
+                            ((fun x => Map.empty x)[{ name := "data" }] ←ₘ (18 : ℕ))[{ name := "in" }] ←ₘ (4 : ℕ),
+                          constraints := [], cycle := (0 : ℕ), felts := Map.empty, isFailed := false,
+                          props := Map.empty,
+                          vars := [{ name := "in" }, { name := "data" }] }[props][{ name := "%6" }] ←
+                        True)[felts][{ name := "%4" }] ←
+                      (4 : Felt))[felts][{ name := "%2" }] ←
+                    (8 : Felt))[felts][{ name := "%1" }] ←
+                  (16 : Felt))[felts][{ name := "%3" }] ←
+                (2 : Felt))[props][{ name := "%28" }] ←
+              x3 -
+                  ((y10 * (64 : Felt) + (y1 * (16 : Felt) + y9 * (8 : Felt) + y8 * (4 : Felt) + y0)) * (2 : Felt) +
+                    y13) =
+                (0 : Felt))[felts][{ name := "%31" }] ←
+            y4 * (4 : Felt))[felts][{ name := "%33" }] ←
+          y2))  := by
     rewrite [part6_cumulative_wp]
     rewrite [part7_updates_opaque]
     unfold part6_state
@@ -51,6 +100,5 @@ lemma part7_cumulative_wp {x0 y0 y1 y2 y3 y4 y5 y6 y7 y8 y9 y10 y11 y12 y13 y14 
     -- 0 sets
     -- rewrite [Map.drop_of_updates]
     -- simp only [Map.drop_base, ne_eq, Map.update_drop_swap, Map.update_drop]
-    rfl
 
 end Risc0.ComputeDecode.Constraints.WP
