Risc0/Gadgets/ComputeDecode/Witness/Code.lean
@@ -143,9 +143,9 @@ def run (st: State) : BufferAtTime :=
 
 end Code
 
-def start_state (input data : BufferAtTime) : State :=
-  { buffers := Map.fromList [(⟨"in"⟩, [input]), (⟨"data"⟩, [data])]
-  , bufferWidths := Map.fromList [(⟨"in"⟩, 128), (⟨"data"⟩, 18)]
+def start_state (input : BufferAtTime) : State :=
+  { buffers := Map.fromList [(⟨"in"⟩, [input]), (⟨"data"⟩, [[none, none, none, none, none, none, none, none, none, none, none, none, none, none, none, none, none, none]])]
+  , bufferWidths := Map.fromList [(⟨"in"⟩, 4), (⟨"data"⟩, 18)]
   , constraints := []
   , cycle := 0
   , felts := Map.empty
