Risc0/Gadgets/ComputeDecode/Constraints/WeakestPresPart16.lean
@@ -1,0 +1,119 @@
+import Risc0.Basic
+import Risc0.MlirTactics
+import Risc0.Gadgets.ComputeDecode.Constraints.Code
+import Risc0.Gadgets.ComputeDecode.Constraints.WeakestPresPart15
+
+namespace Risc0.ComputeDecode.Constraints.WP
+
+open MLIRNotation
+
+-- The state obtained by running Code.part16 on st
+def part16_state (st: State) : State :=
+  
+        (st[props][{ name := "%64" }] ←
+          (Option.get! (State.props st { name := "%58" }) ∧
+            Option.get! (State.felts st { name := "%63" }) = (0 : Felt))) 
+
+def part16_drops (st: State) : State :=
+  State.dropFelts (State.dropFelts (State.dropFelts (State.dropFelts (State.dropFelts (State.dropFelts (st) ⟨"%6"⟩) ⟨"%28"⟩) ⟨"%43"⟩) ⟨"%58"⟩) ⟨"%63"⟩) ⟨"%64"⟩
+
+-- Run the program from part16 onwards by using part16_state rather than Code.part16
+def part16_state_update (st: State): State :=
+  part16_drops (part16_state st)
+
+-- Prove that substituting part16_state for Code.part16 produces the same result
+lemma part16_wp {st : State}:
+  Code.getReturn (MLIR.runProgram (Code.part16;dropfelt ⟨"%6"⟩;dropfelt ⟨"%28"⟩;dropfelt ⟨"%43"⟩;dropfelt ⟨"%58"⟩;dropfelt ⟨"%63"⟩;dropfelt ⟨"%64"⟩) st) ↔
+  Code.getReturn (part16_state_update st) := by
+  unfold MLIR.runProgram; simp only
+  generalize eq : (dropfelt ⟨"%6"⟩;dropfelt ⟨"%28"⟩;dropfelt ⟨"%43"⟩;dropfelt ⟨"%58"⟩;dropfelt ⟨"%63"⟩;dropfelt ⟨"%64"⟩) = prog
+  unfold Code.part16
+  MLIR
+  rewrite [←eq]
+  rewrite [MLIR.run_seq_def,MLIR.run_dropfelt, MLIR.run_seq_def,MLIR.run_dropfelt, MLIR.run_seq_def,MLIR.run_dropfelt, MLIR.run_seq_def,MLIR.run_dropfelt, MLIR.run_seq_def,MLIR.run_dropfelt, MLIR.run_dropfelt]
+  unfold part16_state_update part16_drops part16_state
+  rfl
+
+lemma part16_updates_opaque {st : State} : 
+  Code.getReturn (part15_state_update st) ↔
+  Code.getReturn (part16_state_update (part15_drops (part15_state st))) := by
+  simp [part15_state_update, part16_wp]
+
+lemma part16_cumulative_wp {x0 x1 x2 x3 y0 y1 y2 y3 y4 y5 y6 y7 y8 y9 y10 y11 y12 y13 y14 y15 y16 y17: Felt} :
+  Code.run (start_state [x0,x1,x2,x3] ([y0,y1,y2,y3,y4,y5,y6,y7,y8,y9,y10,y11,y12,y13,y14,y15,y16,y17])) ↔
+  Code.getReturn
+      (part16_state_update
+        ((((({
+                    buffers :=
+                      ((fun x => Map.empty x)[{ name := "data" }] ←ₘ
+                          [[some y0, some y1, some y2, some y3, some y4, some y5, some y6, some y7, some y8, some y9,
+                              some y10, some y11, some y12, some y13, some y14, some y15, some y16,
+                              some y17]])[{ name := "in" }] ←ₘ
+                        [[some x0, some x1, some x2, some x3]],
+                    bufferWidths :=
+                      ((fun x => Map.empty x)[{ name := "data" }] ←ₘ (18 : ℕ))[{ name := "in" }] ←ₘ (4 : ℕ),
+                    constraints := [], cycle := (0 : ℕ), felts := Map.empty, isFailed := false, props := Map.empty,
+                    vars := [{ name := "in" }, { name := "data" }] }[props][{ name := "%6" }] ←
+                  True)[props][{ name := "%28" }] ←
+                x3 -
+                    ((y10 * (64 : Felt) + (y1 * (16 : Felt) + y9 * (8 : Felt) + y8 * (4 : Felt) + y0)) * (2 : Felt) +
+                      y13) =
+                  (0 : Felt))[props][{ name := "%43" }] ←
+              (x3 -
+                    ((y10 * (64 : Felt) + (y1 * (16 : Felt) + y9 * (8 : Felt) + y8 * (4 : Felt) + y0)) * (2 : Felt) +
+                      y13) =
+                  (0 : Felt) ∧
+                x2 - ((y12 * (8 : Felt) + y2 * (2 : Felt) + y11) * (16 : Felt) + y4 * (4 : Felt) + y3) =
+                  (0 : Felt)))[props][{ name := "%58" }] ←
+            ((x3 -
+                    ((y10 * (64 : Felt) + (y1 * (16 : Felt) + y9 * (8 : Felt) + y8 * (4 : Felt) + y0)) * (2 : Felt) +
+                      y13) =
+                  (0 : Felt) ∧
+                x2 - ((y12 * (8 : Felt) + y2 * (2 : Felt) + y11) * (16 : Felt) + y4 * (4 : Felt) + y3) = (0 : Felt)) ∧
+              x1 - (y14 * (128 : Felt) + (y15 * (4 : Felt) + y5) * (16 : Felt) + y7 * (4 : Felt) + y6) =
+                (0 : Felt)))[felts][{ name := "%63" }] ←
+          x0 - (y16 * (128 : Felt) + y17)))  := by
+    rewrite [part15_cumulative_wp]
+    rewrite [part16_updates_opaque]
+    unfold part15_state
+    MLIR_states_updates
+    -- 0 withEqZeros
+    -- rewrite [withEqZero_def]
+    -- MLIR_states_updates
+    unfold part15_drops
+    -- 4 drops
+    simp only [State.drop_update_swap, State.drop_update_same, State.drop_updateProps_swap]
+    rewrite [State.dropFelts]
+    simp only [State.dropFelts_buffers, State.dropFelts_bufferWidths, State.dropFelts_constraints, State.dropFelts_cycle, State.dropFelts_felts, State.dropFelts_isFailed, State.dropFelts_props, State.dropFelts_vars]
+    simp only [Map.drop_base, ne_eq, Map.update_drop_swap, Map.update_drop]
+    -- 0 sets
+    -- rewrite [Map.drop_of_updates]
+    -- simp only [Map.drop_base, ne_eq, Map.update_drop_swap, Map.update_drop]
+
+lemma closed_form {x0 x1 x2 x3 y0 y1 y2 y3 y4 y5 y6 y7 y8 y9 y10 y11 y12 y13 y14 y15 y16 y17: Felt} :
+  Code.run (start_state [x0,x1,x2,x3] ([y0,y1,y2,y3,y4,y5,y6,y7,y8,y9,y10,y11,y12,y13,y14,y15,y16,y17])) ↔
+   ((x3 - ((y10 * (64 : Felt) + (y1 * (16 : Felt) + y9 * (8 : Felt) + y8 * (4 : Felt) + y0)) * (2 : Felt) + y13) =
+            (0 : Felt) ∧
+          x2 - ((y12 * (8 : Felt) + y2 * (2 : Felt) + y11) * (16 : Felt) + y4 * (4 : Felt) + y3) = (0 : Felt)) ∧
+        x1 - (y14 * (128 : Felt) + (y15 * (4 : Felt) + y5) * (16 : Felt) + y7 * (4 : Felt) + y6) = (0 : Felt)) ∧
+      x0 - (y16 * (128 : Felt) + y17) = (0 : Felt)  := by
+    rewrite [part16_cumulative_wp]
+    unfold part16_state_update
+    unfold part16_state
+    MLIR_states_updates
+    -- 0 withEqZeros
+    -- rewrite [withEqZero_def]
+    -- MLIR_states_updates
+    unfold part16_drops
+    -- 6 drops
+    simp only [State.drop_update_swap, State.drop_update_same, State.drop_updateProps_swap]
+    rewrite [State.dropFelts]
+    simp only [State.dropFelts_buffers, State.dropFelts_bufferWidths, State.dropFelts_constraints, State.dropFelts_cycle, State.dropFelts_felts, State.dropFelts_isFailed, State.dropFelts_props, State.dropFelts_vars]
+    simp only [Map.drop_base, ne_eq, Map.update_drop_swap, Map.update_drop]
+    -- 0 sets
+    -- rewrite [Map.drop_of_updates]
+    -- simp only [Map.drop_base, ne_eq, Map.update_drop_swap, Map.update_drop]
+    unfold Code.getReturn
+    simp only
+    simp only [Code.getReturn, State.constraintsInVar, State.updateProps_props_get_wobbly, Option.getD_some]
+end Risc0.ComputeDecode.Constraints.WP
