Risc0/Gadgets/ComputeDecode/Witness/WeakestPresPart15.lean
@@ -1,0 +1,104 @@
+import Risc0.Basic
+import Risc0.MlirTactics
+import Risc0.Gadgets.ComputeDecode.Witness.Code
+import Risc0.Gadgets.ComputeDecode.Witness.WeakestPresPart14
+
+namespace Risc0.ComputeDecode.Witness.WP
+
+open MLIRNotation
+
+-- The state obtained by running Code.part15 on st
+def part15_state (st: State) : State :=
+  
+          ((State.set!
+              ((st[felts][{ name := "%100" }] ←
+                  feltBitAnd (Option.get! (State.felts st { name := "%21" }))
+                    (Option.get! (State.felts st { name := "%6" })))[felts][{ name := "%101" }] ←
+                feltBitAnd (Option.get! (State.felts st { name := "%21" }))
+                    (Option.get! (State.felts st { name := "%6" })) *
+                  Option.get! (State.felts st { name := "%5" }))
+              { name := "data" } (7 : ℕ)
+              (feltBitAnd (Option.get! (State.felts st { name := "%21" }))
+                  (Option.get! (State.felts st { name := "%6" })) *
+                Option.get! (State.felts st { name := "%5" })))[felts][{ name := "%102" }] ←
+            feltBitAnd (Option.get! (State.felts st { name := "%21" }))
+              (Option.get! (State.felts st { name := "%4" }))) 
+
+def part15_drops (st: State) : State :=
+  State.dropFelts (State.dropFelts (State.dropFelts (State.dropFelts (State.dropFelts (st) ⟨"%6"⟩) ⟨"%5"⟩) ⟨"%4"⟩) ⟨"%100"⟩) ⟨"%101"⟩
+
+-- Run the program from part15 onwards by using part15_state rather than Code.part15
+def part15_state_update (st: State): State :=
+  Γ (part15_drops (part15_state st)) ⟦Code.part16;dropfelt ⟨"%18"⟩;dropfelt ⟨"%102"⟩;dropfelt ⟨"%103"⟩;Code.part17;dropfelt ⟨"%104"⟩;dropfelt ⟨"%0"⟩;dropfelt ⟨"%105"⟩;Code.part18;dropfelt ⟨"%26"⟩;Code.part19;dropfelt ⟨"%28"⟩;dropfelt ⟨"%29"⟩;dropfelt ⟨"%30"⟩;dropfelt ⟨"%31"⟩;Code.part20;dropfelt ⟨"%27"⟩;dropfelt ⟨"%32"⟩;dropfelt ⟨"%33"⟩;dropfelt ⟨"%25"⟩;Code.part21;dropfelt ⟨"%3"⟩;dropfelt ⟨"%34"⟩;dropfelt ⟨"%35"⟩;dropfelt ⟨"%36"⟩;dropfelt ⟨"%37"⟩;Code.part22;dropfelt ⟨"%23"⟩;dropfelt ⟨"%38"⟩;dropfelt ⟨"%24"⟩;dropfelt ⟨"%39"⟩;dropfelt ⟨"%40"⟩;Code.part23;dropfelt ⟨"%11"⟩;dropfelt ⟨"%42"⟩;dropfelt ⟨"%45"⟩;Code.part24;dropfelt ⟨"%13"⟩;dropfelt ⟨"%46"⟩;dropfelt ⟨"%47"⟩;dropfelt ⟨"%48"⟩;Code.part25;dropfelt ⟨"%43"⟩;dropfelt ⟨"%49"⟩;dropfelt ⟨"%44"⟩;dropfelt ⟨"%50"⟩;dropfelt ⟨"%51"⟩;Code.part26;dropfelt ⟨"%22"⟩;dropfelt ⟨"%52"⟩;dropfelt ⟨"%41"⟩;dropfelt ⟨"%53"⟩;dropfelt ⟨"%54"⟩;Code.part27;dropfelt ⟨"%7"⟩;dropfelt ⟨"%56"⟩;dropfelt ⟨"%59"⟩;Code.part28;dropfelt ⟨"%15"⟩;dropfelt ⟨"%60"⟩;dropfelt ⟨"%58"⟩;dropfelt ⟨"%61"⟩;dropfelt ⟨"%63"⟩;Code.part29;dropfelt ⟨"%57"⟩;dropfelt ⟨"%62"⟩;dropfelt ⟨"%64"⟩;dropfelt ⟨"%65"⟩;dropfelt ⟨"%66"⟩;dropfelt ⟨"%55"⟩;Code.part30;dropfelt ⟨"%19"⟩;dropfelt ⟨"%21"⟩;dropfelt ⟨"%67"⟩;dropfelt ⟨"%68"⟩;dropfelt ⟨"%70"⟩;Code.part31;dropfelt ⟨"%20"⟩;dropfelt ⟨"%71"⟩;dropfelt ⟨"%69"⟩;dropfelt ⟨"%72"⟩;dropfelt ⟨"%73"⟩⟧
+
+-- Prove that substituting part15_state for Code.part15 produces the same result
+lemma part15_wp {st : State} {y0 y1 y2 y3 y4 y5 y6 y7 y8 y9 y10 y11 y12 y13 y14 y15 y16 y17 : Option Felt} :
+  Code.getReturn (MLIR.runProgram (Code.part15;dropfelt ⟨"%6"⟩;dropfelt ⟨"%5"⟩;dropfelt ⟨"%4"⟩;dropfelt ⟨"%100"⟩;dropfelt ⟨"%101"⟩;Code.part16;dropfelt ⟨"%18"⟩;dropfelt ⟨"%102"⟩;dropfelt ⟨"%103"⟩;Code.part17;dropfelt ⟨"%104"⟩;dropfelt ⟨"%0"⟩;dropfelt ⟨"%105"⟩;Code.part18;dropfelt ⟨"%26"⟩;Code.part19;dropfelt ⟨"%28"⟩;dropfelt ⟨"%29"⟩;dropfelt ⟨"%30"⟩;dropfelt ⟨"%31"⟩;Code.part20;dropfelt ⟨"%27"⟩;dropfelt ⟨"%32"⟩;dropfelt ⟨"%33"⟩;dropfelt ⟨"%25"⟩;Code.part21;dropfelt ⟨"%3"⟩;dropfelt ⟨"%34"⟩;dropfelt ⟨"%35"⟩;dropfelt ⟨"%36"⟩;dropfelt ⟨"%37"⟩;Code.part22;dropfelt ⟨"%23"⟩;dropfelt ⟨"%38"⟩;dropfelt ⟨"%24"⟩;dropfelt ⟨"%39"⟩;dropfelt ⟨"%40"⟩;Code.part23;dropfelt ⟨"%11"⟩;dropfelt ⟨"%42"⟩;dropfelt ⟨"%45"⟩;Code.part24;dropfelt ⟨"%13"⟩;dropfelt ⟨"%46"⟩;dropfelt ⟨"%47"⟩;dropfelt ⟨"%48"⟩;Code.part25;dropfelt ⟨"%43"⟩;dropfelt ⟨"%49"⟩;dropfelt ⟨"%44"⟩;dropfelt ⟨"%50"⟩;dropfelt ⟨"%51"⟩;Code.part26;dropfelt ⟨"%22"⟩;dropfelt ⟨"%52"⟩;dropfelt ⟨"%41"⟩;dropfelt ⟨"%53"⟩;dropfelt ⟨"%54"⟩;Code.part27;dropfelt ⟨"%7"⟩;dropfelt ⟨"%56"⟩;dropfelt ⟨"%59"⟩;Code.part28;dropfelt ⟨"%15"⟩;dropfelt ⟨"%60"⟩;dropfelt ⟨"%58"⟩;dropfelt ⟨"%61"⟩;dropfelt ⟨"%63"⟩;Code.part29;dropfelt ⟨"%57"⟩;dropfelt ⟨"%62"⟩;dropfelt ⟨"%64"⟩;dropfelt ⟨"%65"⟩;dropfelt ⟨"%66"⟩;dropfelt ⟨"%55"⟩;Code.part30;dropfelt ⟨"%19"⟩;dropfelt ⟨"%21"⟩;dropfelt ⟨"%67"⟩;dropfelt ⟨"%68"⟩;dropfelt ⟨"%70"⟩;Code.part31;dropfelt ⟨"%20"⟩;dropfelt ⟨"%71"⟩;dropfelt ⟨"%69"⟩;dropfelt ⟨"%72"⟩;dropfelt ⟨"%73"⟩) st) = [y0, y1, y2, y3, y4, y5, y6, y7, y8, y9, y10, y11, y12, y13, y14, y15, y16, y17] ↔
+  Code.getReturn (part15_state_update st) = [y0, y1, y2, y3, y4, y5, y6, y7, y8, y9, y10, y11, y12, y13, y14, y15, y16, y17] := by
+  unfold MLIR.runProgram; simp only
+  generalize eq : (dropfelt ⟨"%6"⟩;dropfelt ⟨"%5"⟩;dropfelt ⟨"%4"⟩;dropfelt ⟨"%100"⟩;dropfelt ⟨"%101"⟩;Code.part16;dropfelt ⟨"%18"⟩;dropfelt ⟨"%102"⟩;dropfelt ⟨"%103"⟩;Code.part17;dropfelt ⟨"%104"⟩;dropfelt ⟨"%0"⟩;dropfelt ⟨"%105"⟩;Code.part18;dropfelt ⟨"%26"⟩;Code.part19;dropfelt ⟨"%28"⟩;dropfelt ⟨"%29"⟩;dropfelt ⟨"%30"⟩;dropfelt ⟨"%31"⟩;Code.part20;dropfelt ⟨"%27"⟩;dropfelt ⟨"%32"⟩;dropfelt ⟨"%33"⟩;dropfelt ⟨"%25"⟩;Code.part21;dropfelt ⟨"%3"⟩;dropfelt ⟨"%34"⟩;dropfelt ⟨"%35"⟩;dropfelt ⟨"%36"⟩;dropfelt ⟨"%37"⟩;Code.part22;dropfelt ⟨"%23"⟩;dropfelt ⟨"%38"⟩;dropfelt ⟨"%24"⟩;dropfelt ⟨"%39"⟩;dropfelt ⟨"%40"⟩;Code.part23;dropfelt ⟨"%11"⟩;dropfelt ⟨"%42"⟩;dropfelt ⟨"%45"⟩;Code.part24;dropfelt ⟨"%13"⟩;dropfelt ⟨"%46"⟩;dropfelt ⟨"%47"⟩;dropfelt ⟨"%48"⟩;Code.part25;dropfelt ⟨"%43"⟩;dropfelt ⟨"%49"⟩;dropfelt ⟨"%44"⟩;dropfelt ⟨"%50"⟩;dropfelt ⟨"%51"⟩;Code.part26;dropfelt ⟨"%22"⟩;dropfelt ⟨"%52"⟩;dropfelt ⟨"%41"⟩;dropfelt ⟨"%53"⟩;dropfelt ⟨"%54"⟩;Code.part27;dropfelt ⟨"%7"⟩;dropfelt ⟨"%56"⟩;dropfelt ⟨"%59"⟩;Code.part28;dropfelt ⟨"%15"⟩;dropfelt ⟨"%60"⟩;dropfelt ⟨"%58"⟩;dropfelt ⟨"%61"⟩;dropfelt ⟨"%63"⟩;Code.part29;dropfelt ⟨"%57"⟩;dropfelt ⟨"%62"⟩;dropfelt ⟨"%64"⟩;dropfelt ⟨"%65"⟩;dropfelt ⟨"%66"⟩;dropfelt ⟨"%55"⟩;Code.part30;dropfelt ⟨"%19"⟩;dropfelt ⟨"%21"⟩;dropfelt ⟨"%67"⟩;dropfelt ⟨"%68"⟩;dropfelt ⟨"%70"⟩;Code.part31;dropfelt ⟨"%20"⟩;dropfelt ⟨"%71"⟩;dropfelt ⟨"%69"⟩;dropfelt ⟨"%72"⟩;dropfelt ⟨"%73"⟩) = prog
+  unfold Code.part15
+  MLIR
+  rewrite [←eq]
+  rewrite [MLIR.run_seq_def,MLIR.run_dropfelt, MLIR.run_seq_def,MLIR.run_dropfelt, MLIR.run_seq_def,MLIR.run_dropfelt, MLIR.run_seq_def,MLIR.run_dropfelt, MLIR.run_seq_def,MLIR.run_dropfelt]
+  unfold part15_state_update part15_drops part15_state
+  rfl
+
+lemma part15_updates_opaque {st : State} : 
+  Code.getReturn (part14_state_update st) = [y0, y1, y2, y3, y4, y5, y6, y7, y8, y9, y10, y11, y12, y13, y14, y15, y16, y17] ↔
+  Code.getReturn (part15_state_update (part14_drops (part14_state st))) = [y0, y1, y2, y3, y4, y5, y6, y7, y8, y9, y10, y11, y12, y13, y14, y15, y16, y17] := by
+  simp [part14_state_update, part15_wp]
+
+lemma part15_cumulative_wp {x0 x1 x2 x3: Felt} :
+  Code.run (start_state [x0,x1,x2,x3]) = [y0,y1,y2,y3,y4,y5,y6,y7,y8,y9,y10,y11,y12,y13,y14,y15,y16,y17] ↔
+  Code.getReturn
+        (part15_state_update
+          {
+            buffers :=
+              (Map.empty[{ name := "in" }] ←ₘ [[some x0, some x1, some x2, some x3]])[{ name := "data" }] ←ₘ
+                [[some (feltBitAnd x3 (6 : Felt) * (1006632961 : Felt)),
+                    some (feltBitAnd x3 (96 : Felt) * (1950351361 : Felt)),
+                    some (feltBitAnd x2 (96 : Felt) * (1950351361 : Felt)), some (feltBitAnd x2 (3 : Felt)),
+                    some (feltBitAnd x2 (12 : Felt) * (1509949441 : Felt)),
+                    some (feltBitAnd x1 (48 : Felt) * (1887436801 : Felt)), none, none,
+                    some (feltBitAnd x3 (8 : Felt) * (1761607681 : Felt)),
+                    some (feltBitAnd x3 (16 : Felt) * (1887436801 : Felt)),
+                    some (feltBitAnd x3 (128 : Felt) * (1997537281 : Felt)),
+                    some (feltBitAnd x2 (16 : Felt) * (1887436801 : Felt)),
+                    some (feltBitAnd x2 (128 : Felt) * (1997537281 : Felt)), some (feltBitAnd x3 (1 : Felt)),
+                    some (feltBitAnd x1 (128 : Felt) * (1997537281 : Felt)),
+                    some (feltBitAnd x1 (64 : Felt) * (1981808641 : Felt)), none, none]],
+            bufferWidths := ((fun x => Map.empty x)[{ name := "data" }] ←ₘ (18 : ℕ))[{ name := "in" }] ←ₘ (4 : ℕ),
+            constraints := [], cycle := (0 : ℕ),
+            felts :=
+              ((((((((((Map.empty[{ name := "%19" }] ←ₘ (128 : Felt))[{ name := "%23" }] ←ₘ x3)[{ name := "%18" }] ←ₘ
+                                (1997537281 : Felt))[{ name := "%15" }] ←ₘ
+                              (16 : Felt))[{ name := "%13" }] ←ₘ
+                            (8 : Felt))[{ name := "%22" }] ←ₘ
+                          x2)[{ name := "%6" }] ←ₘ
+                        (12 : Felt))[{ name := "%5" }] ←ₘ
+                      (1509949441 : Felt))[{ name := "%4" }] ←ₘ
+                    (3 : Felt))[{ name := "%21" }] ←ₘ
+                  x1)[{ name := "%3" }] ←ₘ
+                (64 : Felt),
+            isFailed := false, props := Map.empty, vars := [{ name := "in" }, { name := "data" }] }) =
+      [y0, y1, y2, y3, y4, y5, y6, y7, y8, y9, y10, y11, y12, y13, y14, y15, y16, y17]  := by
+    rewrite [part14_cumulative_wp]
+    rewrite [part15_updates_opaque]
+    unfold part14_state
+    try simplify_get_hack
+    MLIR_states_updates
+    -- 0 withEqZeros
+    -- rewrite [withEqZero_def]
+    -- MLIR_states_updates
+    unfold part14_drops
+    -- 4 drops
+    simp only [State.drop_update_swap, State.drop_update_same]
+    rewrite [State.dropFelts]
+    simp only [State.dropFelts_buffers, State.dropFelts_bufferWidths, State.dropFelts_constraints, State.dropFelts_cycle, State.dropFelts_felts, State.dropFelts_isFailed, State.dropFelts_props, State.dropFelts_vars]
+    simp only [Map.drop_base, ne_eq, Map.update_drop_swap, Map.update_drop]
+    -- 1 set
+    rewrite [Map.drop_of_updates]
+    simp only [Map.drop_base, ne_eq, Map.update_drop_swap, Map.update_drop]
+
+end Risc0.ComputeDecode.Witness.WP
