Risc0/Gadgets/ComputeDecode/Witness/WeakestPresPart24.lean
@@ -1,0 +1,113 @@
+import Risc0.Basic
+import Risc0.MlirTactics
+import Risc0.Gadgets.ComputeDecode.Witness.Code
+import Risc0.Gadgets.ComputeDecode.Witness.WeakestPresPart23
+
+namespace Risc0.ComputeDecode.Witness.WP
+
+open MLIRNotation
+
+-- The state obtained by running Code.part24 on st
+def part24_state (st: State) : State :=
+  
+          ((((st["%47"] ←ₛ getImpl st { name := "data" } (0 : Back) (12 : ℕ))[felts][{ name := "%48" }] ←
+                Option.get!
+                    (State.felts (st["%47"] ←ₛ getImpl st { name := "data" } (0 : Back) (12 : ℕ)) { name := "%47" }) *
+                  Option.get! (State.felts st { name := "%13" }))[felts][{ name := "%49" }] ←
+              Option.get!
+                    (State.felts (st["%47"] ←ₛ getImpl st { name := "data" } (0 : Back) (12 : ℕ)) { name := "%47" }) *
+                  Option.get! (State.felts st { name := "%13" }) +
+                Option.get! (State.felts st { name := "%46" }))["%44"] ←ₛ
+            getImpl st { name := "data" } (0 : Back) (11 : ℕ)) 
+
+def part24_drops (st: State) : State :=
+  State.dropFelts (State.dropFelts (State.dropFelts (State.dropFelts (st) ⟨"%13"⟩) ⟨"%46"⟩) ⟨"%47"⟩) ⟨"%48"⟩
+
+-- Run the program from part24 onwards by using part24_state rather than Code.part24
+def part24_state_update (st: State): State :=
+  Γ (part24_drops (part24_state st)) ⟦Code.part25;dropfelt ⟨"%43"⟩;dropfelt ⟨"%49"⟩;dropfelt ⟨"%44"⟩;dropfelt ⟨"%50"⟩;dropfelt ⟨"%51"⟩;Code.part26;dropfelt ⟨"%22"⟩;dropfelt ⟨"%52"⟩;dropfelt ⟨"%41"⟩;dropfelt ⟨"%53"⟩;dropfelt ⟨"%54"⟩;Code.part27;dropfelt ⟨"%7"⟩;dropfelt ⟨"%56"⟩;dropfelt ⟨"%59"⟩;Code.part28;dropfelt ⟨"%15"⟩;dropfelt ⟨"%60"⟩;dropfelt ⟨"%58"⟩;dropfelt ⟨"%61"⟩;dropfelt ⟨"%63"⟩;Code.part29;dropfelt ⟨"%57"⟩;dropfelt ⟨"%62"⟩;dropfelt ⟨"%64"⟩;dropfelt ⟨"%65"⟩;dropfelt ⟨"%66"⟩;dropfelt ⟨"%55"⟩;Code.part30;dropfelt ⟨"%19"⟩;dropfelt ⟨"%21"⟩;dropfelt ⟨"%67"⟩;dropfelt ⟨"%68"⟩;dropfelt ⟨"%70"⟩;Code.part31;dropfelt ⟨"%20"⟩;dropfelt ⟨"%71"⟩;dropfelt ⟨"%69"⟩;dropfelt ⟨"%72"⟩;dropfelt ⟨"%73"⟩⟧
+
+-- Prove that substituting part24_state for Code.part24 produces the same result
+lemma part24_wp {st : State} {y0 y1 y2 y3 y4 y5 y6 y7 y8 y9 y10 y11 y12 y13 y14 y15 y16 y17 : Option Felt} :
+  Code.getReturn (MLIR.runProgram (Code.part24;dropfelt ⟨"%13"⟩;dropfelt ⟨"%46"⟩;dropfelt ⟨"%47"⟩;dropfelt ⟨"%48"⟩;Code.part25;dropfelt ⟨"%43"⟩;dropfelt ⟨"%49"⟩;dropfelt ⟨"%44"⟩;dropfelt ⟨"%50"⟩;dropfelt ⟨"%51"⟩;Code.part26;dropfelt ⟨"%22"⟩;dropfelt ⟨"%52"⟩;dropfelt ⟨"%41"⟩;dropfelt ⟨"%53"⟩;dropfelt ⟨"%54"⟩;Code.part27;dropfelt ⟨"%7"⟩;dropfelt ⟨"%56"⟩;dropfelt ⟨"%59"⟩;Code.part28;dropfelt ⟨"%15"⟩;dropfelt ⟨"%60"⟩;dropfelt ⟨"%58"⟩;dropfelt ⟨"%61"⟩;dropfelt ⟨"%63"⟩;Code.part29;dropfelt ⟨"%57"⟩;dropfelt ⟨"%62"⟩;dropfelt ⟨"%64"⟩;dropfelt ⟨"%65"⟩;dropfelt ⟨"%66"⟩;dropfelt ⟨"%55"⟩;Code.part30;dropfelt ⟨"%19"⟩;dropfelt ⟨"%21"⟩;dropfelt ⟨"%67"⟩;dropfelt ⟨"%68"⟩;dropfelt ⟨"%70"⟩;Code.part31;dropfelt ⟨"%20"⟩;dropfelt ⟨"%71"⟩;dropfelt ⟨"%69"⟩;dropfelt ⟨"%72"⟩;dropfelt ⟨"%73"⟩) st) = [y0, y1, y2, y3, y4, y5, y6, y7, y8, y9, y10, y11, y12, y13, y14, y15, y16, y17] ↔
+  Code.getReturn (part24_state_update st) = [y0, y1, y2, y3, y4, y5, y6, y7, y8, y9, y10, y11, y12, y13, y14, y15, y16, y17] := by
+  unfold MLIR.runProgram; simp only
+  generalize eq : (dropfelt ⟨"%13"⟩;dropfelt ⟨"%46"⟩;dropfelt ⟨"%47"⟩;dropfelt ⟨"%48"⟩;Code.part25;dropfelt ⟨"%43"⟩;dropfelt ⟨"%49"⟩;dropfelt ⟨"%44"⟩;dropfelt ⟨"%50"⟩;dropfelt ⟨"%51"⟩;Code.part26;dropfelt ⟨"%22"⟩;dropfelt ⟨"%52"⟩;dropfelt ⟨"%41"⟩;dropfelt ⟨"%53"⟩;dropfelt ⟨"%54"⟩;Code.part27;dropfelt ⟨"%7"⟩;dropfelt ⟨"%56"⟩;dropfelt ⟨"%59"⟩;Code.part28;dropfelt ⟨"%15"⟩;dropfelt ⟨"%60"⟩;dropfelt ⟨"%58"⟩;dropfelt ⟨"%61"⟩;dropfelt ⟨"%63"⟩;Code.part29;dropfelt ⟨"%57"⟩;dropfelt ⟨"%62"⟩;dropfelt ⟨"%64"⟩;dropfelt ⟨"%65"⟩;dropfelt ⟨"%66"⟩;dropfelt ⟨"%55"⟩;Code.part30;dropfelt ⟨"%19"⟩;dropfelt ⟨"%21"⟩;dropfelt ⟨"%67"⟩;dropfelt ⟨"%68"⟩;dropfelt ⟨"%70"⟩;Code.part31;dropfelt ⟨"%20"⟩;dropfelt ⟨"%71"⟩;dropfelt ⟨"%69"⟩;dropfelt ⟨"%72"⟩;dropfelt ⟨"%73"⟩) = prog
+  unfold Code.part24
+  MLIR
+  rewrite [←eq]
+  rewrite [MLIR.run_seq_def,MLIR.run_dropfelt, MLIR.run_seq_def,MLIR.run_dropfelt, MLIR.run_seq_def,MLIR.run_dropfelt, MLIR.run_seq_def,MLIR.run_dropfelt]
+  unfold part24_state_update part24_drops part24_state
+  rfl
+
+lemma part24_updates_opaque {st : State} : 
+  Code.getReturn (part23_state_update st) = [y0, y1, y2, y3, y4, y5, y6, y7, y8, y9, y10, y11, y12, y13, y14, y15, y16, y17] ↔
+  Code.getReturn (part24_state_update (part23_drops (part23_state st))) = [y0, y1, y2, y3, y4, y5, y6, y7, y8, y9, y10, y11, y12, y13, y14, y15, y16, y17] := by
+  simp [part23_state_update, part24_wp]
+
+lemma part24_cumulative_wp {x0 x1 x2 x3: Felt} :
+  Code.run (start_state [x0,x1,x2,x3]) = [y0,y1,y2,y3,y4,y5,y6,y7,y8,y9,y10,y11,y12,y13,y14,y15,y16,y17] ↔
+  Code.getReturn
+        (part24_state_update
+          (({
+                buffers :=
+                  ((fun x => Map.empty x)[{ name := "in" }] ←ₘ
+                      [[some x0, some x1, some x2, some x3]])[{ name := "data" }] ←ₘ
+                    [[some (feltBitAnd x3 (6 : Felt) * (1006632961 : Felt)),
+                        some (feltBitAnd x3 (96 : Felt) * (1950351361 : Felt)),
+                        some (feltBitAnd x2 (96 : Felt) * (1950351361 : Felt)), some (feltBitAnd x2 (3 : Felt)),
+                        some (feltBitAnd x2 (12 : Felt) * (1509949441 : Felt)),
+                        some (feltBitAnd x1 (48 : Felt) * (1887436801 : Felt)), some (feltBitAnd x1 (3 : Felt)),
+                        some (feltBitAnd x1 (12 : Felt) * (1509949441 : Felt)),
+                        some (feltBitAnd x3 (8 : Felt) * (1761607681 : Felt)),
+                        some (feltBitAnd x3 (16 : Felt) * (1887436801 : Felt)),
+                        some (feltBitAnd x3 (128 : Felt) * (1997537281 : Felt)),
+                        some (feltBitAnd x2 (16 : Felt) * (1887436801 : Felt)),
+                        some (feltBitAnd x2 (128 : Felt) * (1997537281 : Felt)), some (feltBitAnd x3 (1 : Felt)),
+                        some (feltBitAnd x1 (128 : Felt) * (1997537281 : Felt)),
+                        some (feltBitAnd x1 (64 : Felt) * (1981808641 : Felt)),
+                        some (feltBitAnd x0 (128 : Felt) * (1997537281 : Felt)), some (feltBitAnd x0 (127 : Felt))]],
+                bufferWidths := ((fun x => Map.empty x)[{ name := "data" }] ←ₘ (18 : ℕ))[{ name := "in" }] ←ₘ (4 : ℕ),
+                constraints :=
+                  [x3 -
+                        ((feltBitAnd x3 (128 : Felt) * (1997537281 : Felt) * (64 : Felt) +
+                              (feltBitAnd x3 (96 : Felt) * (1950351361 : Felt) * (16 : Felt) +
+                                    feltBitAnd x3 (16 : Felt) * (1887436801 : Felt) * (8 : Felt) +
+                                  feltBitAnd x3 (8 : Felt) * (1761607681 : Felt) * (4 : Felt) +
+                                feltBitAnd x3 (6 : Felt) * (1006632961 : Felt))) *
+                            (2 : Felt) +
+                          feltBitAnd x3 (1 : Felt)) =
+                      (0 : Felt)],
+                cycle := (0 : ℕ),
+                felts :=
+                  ((((((Map.empty[{ name := "%19" }] ←ₘ (128 : Felt))[{ name := "%15" }] ←ₘ
+                              (16 : Felt))[{ name := "%13" }] ←ₘ
+                            (8 : Felt))[{ name := "%22" }] ←ₘ
+                          x2)[{ name := "%21" }] ←ₘ
+                        x1)[{ name := "%20" }] ←ₘ
+                      x0)[{ name := "%7" }] ←ₘ
+                    (4 : Felt),
+                isFailed := false, props := Map.empty,
+                vars := [{ name := "in" }, { name := "data" }] }[felts][{ name := "%43" }] ←
+              feltBitAnd x2 (12 : Felt) * (1509949441 : Felt) * (4 : Felt))[felts][{ name := "%46" }] ←
+            feltBitAnd x2 (96 : Felt) * (1950351361 : Felt) * (2 : Felt))) =
+      [y0, y1, y2, y3, y4, y5, y6, y7, y8, y9, y10, y11, y12, y13, y14, y15, y16, y17]  := by
+    rewrite [part23_cumulative_wp]
+    rewrite [part24_updates_opaque]
+    unfold part23_state
+    try simplify_get_hack
+    MLIR_states_updates
+    -- 0 withEqZeros
+    -- rewrite [withEqZero_def]
+    -- MLIR_states_updates
+    unfold part23_drops
+    -- 3 drops
+    simp only [State.drop_update_swap, State.drop_update_same]
+    rewrite [State.dropFelts]
+    simp only [State.dropFelts_buffers, State.dropFelts_bufferWidths, State.dropFelts_constraints, State.dropFelts_cycle, State.dropFelts_felts, State.dropFelts_isFailed, State.dropFelts_props, State.dropFelts_vars]
+    simp only [Map.drop_base, ne_eq, Map.update_drop_swap, Map.update_drop]
+    -- 0 sets
+    -- rewrite [Map.drop_of_updates]
+    -- simp only [Map.drop_base, ne_eq, Map.update_drop_swap, Map.update_drop]
+
+end Risc0.ComputeDecode.Witness.WP
